src/basic/FStar.Options.fsti
@@ -183,6 +183,7 @@ val print_implicits             : unit    -> bool
 val print_real_names            : unit    -> bool
 val print_universes             : unit    -> bool
 val print_z3_statistics         : unit    -> bool
+val proof_recovery              : unit    -> bool
 val quake_lo                    : unit    -> int
 val quake_hi                    : unit    -> int
 val quake_keep                  : unit    -> bool
